src/QUIC.Impl.fsti
@@ -381,3 +381,6 @@ val decrypt: #i:G.erased index -> (
             == QUIC.Spec.Success (U8.v r.pn_len) (U64.v r.pn) (g_header r.header h1) plain)))
       | _ ->
           False))
+
+(* for extraction testing purposes only *)
+val filter_packet_header_byte: U8.t -> Tot bool
